studies/falcon-deadlock/StudyFalconDeadlock.lean
@@ -1,2 +1,3 @@
 import TwoPeerLoadStore
 import PullAckStudy
+import ProactiveRxStudy
